GNF: added one direction of equivalence proof for G1 and G2

Gschossmann/GNF.thy
@@ -1,6 +1,24 @@
 theory GNF
-  imports cfg_renaming cfg_merging util derivel_nts cfg_util map_tms
+  imports cfg_renaming cfg_merging util derivel_nts cfg_util map_tms cnf_induct
 begin
+
+
+(* currently, only one direction is proven (apart from a few sorries for small proofs) *)
+(* The core of the proof needs plenty of garbage collection and redesign *)
+(* Especially, it would be easier to show the equivalence of G0 and G2 directly, without G1,
+   which saves a lot of tinkering with Original / Renamed
+*)
+
+(* CNF.thy? *)
+definition some_cnf :: "('n::infinite,'t) cfg \<Rightarrow> ('n,'t) cfg" where
+  "some_cnf G = (SOME G'. (cnf G') \<and> (L G' = L G - {[]}))"
+
+(* CNF.thy? *)
+lemma some_cnf_cnf: "cnf (some_cnf (G::('n::infinite,'t) cfg)) \<and> L (some_cnf G) = L G - {[]}"
+proof -
+  from cnf_exists have "\<exists>(G'::('n::infinite,'t) cfg). cnf G' \<and> L G' = L G - {[]}" by blast
+  then show ?thesis unfolding some_cnf_def by (rule someI_ex)
+qed
 
 
 abbreviation "gnf_rhs rhs \<equiv> (\<exists>t nts. rhs = Tm t # map Nt nts)"
@@ -11,14 +29,20 @@ definition GNF :: "('n, 't) Prods \<Rightarrow> bool" where
 abbreviation gnf :: "('n, 't) cfg \<Rightarrow> bool" where
   "gnf G \<equiv> GNF (set (prods G))"
 
-definition "R P (A::'n) (a::'t) = {\<beta>. P \<turnstile> [Nt A] \<Rightarrow>l* ((Tm a) # map Nt \<beta>)}"
+
+
+lemma map_rename_syms: "map Nt (map f xs) = rename_syms f (map Nt xs)"
+  by simp
+
+
+definition "R_func P (A::'n) (a::'t) = {\<beta>. P \<turnstile> [Nt A] \<Rightarrow>l* ((Tm a) # map Nt \<beta>)}"
 
 (* properties that G_A,a has *)
-definition "G_props (A::'n) (a::'t) G G0 = (L G = R (set (prods G0)) A a \<and> rlin2 (set (prods G)))"
+definition "G_props (A::'n) (a::'t) G0 G = (L G = R_func (set (prods G0)) A a \<and> rlin2 (set (prods G)))"
 
-lemma exists_rlin_G_for_R: "cnf G0 \<Longrightarrow> (\<And>A a. (\<exists>G. G_props A a G G0))"
+lemma exists_G_for_R: "cnf G0 \<Longrightarrow> (\<And>A a. (\<exists>G. G_props A a G0 G))"
   (* 
-      They Grammar {A' \<longrightarrow> B'C | A \<longrightarrow> BC @ P} \<union> {A' \<longrightarrow> \<epsilon> | A \<longrightarrow> a \<in> P}
+      The Grammar {A' \<longrightarrow> B'C | A \<longrightarrow> BC @ P} \<union> {A' \<longrightarrow> \<epsilon> | A \<longrightarrow> a \<in> P}
       produces the language  R (set (prods G0)) A a
       see Kozen. Automata and Computability pp Lecture 21 (about GNF)
 
@@ -29,12 +53,216 @@ lemma exists_rlin_G_for_R: "cnf G0 \<Longrightarrow> (\<And>A a. (\<exists>G. G_
    *)
   sorry
 
+
+
+
+definition "some_G_for_R (A::'n) (a::'t) G0 \<equiv> 
+  SOME G. G_props A a G0 G"
+
+lemma some_G_for_R_props:
+  assumes "cnf G0"
+    shows "G_props A a G0 (some_G_for_R A a G0)"
+proof -
+  from assms have "\<exists>G. G_props A a G0 G" using exists_G_for_R by fast
+  then show "G_props A a G0 (some_G_for_R A a G0)"
+    unfolding some_G_for_R_def G_props_def by (rule someI_ex)
+qed
+
+lemma some_G_for_R_Lang: "cnf G0 \<Longrightarrow> L (some_G_for_R A a G0) = R_func (set (prods G0)) A a"
+  using some_G_for_R_props unfolding G_props_def by fast
+
+lemma some_G_for_R_rlin2: "cnf G0 \<Longrightarrow> rlin2 (set (prods (some_G_for_R A a G0)))"
+  using some_G_for_R_props unfolding G_props_def by fast
+
+
+
 datatype ('n, 't) renamed = Original 'n | Renamed 'n 't nat
+
+lemma inj_Original: "inj Original"
+  unfolding inj_def by blast
 
 definition "removed_from_G2 P = (\<exists>X B Y. (X, [Nt (Original B), Nt Y]) = P)"
 
 definition "original_sym s \<equiv> (\<exists>nt. s = Nt (Original nt)) \<or> (\<exists>tm. s = Tm tm)"
 abbreviation "original_syms ss \<equiv> \<forall>s \<in> (set ss). original_sym s"  
+
+
+
+lemma derivel_not_elim_tm:
+  assumes "P \<turnstile> xs \<Rightarrow>l map Nt ys"
+  shows "\<exists>xs'. xs = map Nt xs'"
+proof -
+  from assms have "(\<exists>(A, w)\<in>P. \<exists>u1 u2. xs = map Tm u1 @ Nt A # u2 \<and> map Nt ys = map Tm u1 @ w @ u2)"
+    by (simp only: derivel_iff)
+  then obtain A w u1 u2 where
+         A_w: "(A, w)\<in>P"
+      and xs: "xs = map Tm u1 @ Nt A # u2"
+      and ys: "map Nt ys = map Tm u1 @ w @ u2"
+    by fast
+
+  from ys have u1: "u1 = []"
+    by (metis Nil_is_append_conv Nil_is_map_conv hd_append list.map_sel(1) sym.simps(4))
+  moreover from ys obtain u2' where "u2 = map Nt u2'"
+    by (metis append_eq_map_conv)
+
+  ultimately have "xs = map Nt (A # u2')"
+    by (simp add: xs)
+  then show ?thesis by blast
+qed
+
+lemma deriveln_not_elim_tm:
+  assumes "P \<turnstile> xs \<Rightarrow>l(n) map Nt ys"
+  shows "\<exists>xs'. xs = map Nt xs'"
+using assms
+proof (induction n arbitrary: xs)
+  case 0
+  then show ?case by auto
+next
+  case (Suc n)
+  then obtain z where "P \<turnstile> xs \<Rightarrow>l z" and "P \<turnstile> z \<Rightarrow>l(n) map Nt ys"
+    using relpowp_Suc_E2 by metis
+  with Suc show ?case using derivel_not_elim_tm
+    by blast
+qed
+
+
+lemma derivel_nts_suffix:
+  assumes "P \<turnstile> Nt X # map Nt Xs \<Rightarrow>l map Nt Ys"
+  shows "\<exists>Ys'. Ys' @ Xs = Ys \<and> P \<turnstile> [Nt X] \<Rightarrow>l map Nt Ys'"
+proof -
+  from \<open>P \<turnstile> Nt X # map Nt Xs \<Rightarrow>l map Nt Ys\<close> have
+      "\<exists>(A, w)\<in>P. \<exists>u1 u2. Nt X # map Nt Xs = map Tm u1 @ Nt A # u2 \<and> map Nt Ys = map Tm u1 @ w @ u2"
+    by (simp only: derivel_iff)
+  then obtain A w u1 u2 where
+           A_w: "(A, w)\<in>P"
+      and X_Xs: "Nt X # map Nt Xs = map Tm u1 @ Nt A # u2"
+      and Ys: "map Nt Ys = map Tm u1 @ w @ u2"
+    by fast
+
+  from X_Xs have u1: "u1 = []"
+    by (metis (no_types, opaque_lifting) Cons_eq_append_conv list.map_disc_iff map_eq_Cons_D sym.distinct(1))
+  moreover from u1 X_Xs obtain u2' where u2':"u2 = map Nt u2'"
+    by auto
+  moreover note X_Xs
+  ultimately have "Nt X # map Nt Xs = map Nt (A # u2')"
+    by (smt (verit, best) append_self_conv2 list.inj_map_strong list.simps(9) map_is_Nil_conv slemma4_2_0)
+  then have "map Nt (X # Xs) = map Nt (A # u2')" by simp
+  then have "X # Xs = A # u2'"
+    by (metis list.inj_map_strong sym.inject(1))
+  then have "X = A" and "Xs = u2'" by auto
+
+  from u1 Ys obtain w' where "w = map Nt w'"
+    by (metis append_eq_map_conv)
+
+  with Ys have "map Nt Ys = map Tm u1 @ map Nt w' @ u2"
+    by simp
+  with u1 have "map Nt Ys = map Tm [] @ map Nt w' @ u2"
+    by simp
+  then have "map Nt Ys = map Nt w' @ u2"
+    by simp
+  with u2' have "map Nt Ys = map Nt w' @ map Nt u2'"
+    by (metis list.inj_map_strong map_append sym.inject(1))
+  with \<open>Xs = u2'\<close> have "map Nt Ys = map Nt w' @ map Nt Xs"
+    by simp
+  then have "w' @ Xs = Ys"
+    by (metis list.inj_map_strong map_append sym.inject(1))
+
+  moreover from A_w have "P \<turnstile> [Nt A] \<Rightarrow>l w"
+    by (simp add: derivel_Nt_Cons)
+  with A_w have "P \<turnstile> [Nt X] \<Rightarrow>l w"
+    using \<open>X = A\<close> by blast
+  with A_w \<open>w = map Nt w'\<close> have "P \<turnstile> [Nt X] \<Rightarrow>l map Nt w'"
+    by blast
+
+  ultimately have "w' @ Xs = Ys \<and> P \<turnstile> [Nt X] \<Rightarrow>l map Nt w'"
+    by simp
+  then show ?thesis by fast
+qed
+
+
+lemma Eps_free_derivels_Nil: "Eps_free R \<Longrightarrow> R \<turnstile> l \<Rightarrow>l* [] \<longleftrightarrow> l = []"
+  by (meson Eps_free_derives_Nil derivels_from_empty derivels_imp_derives)
+
+
+lemma CNF_Eps_free: "CNF P \<Longrightarrow> Eps_free P"
+  unfolding CNF_def Eps_free_def by blast
+
+
+lemma deriveln_nts_suffix:
+  assumes "P \<turnstile> Nt X # map Nt Xs \<Rightarrow>l(n) map Nt Ys"
+  assumes "Eps_free P"
+  shows "\<exists>Ys'. Ys' @ Xs = Ys \<and> P \<turnstile> [Nt X] \<Rightarrow>l(n) map Nt Ys'"
+using assms
+proof (induction n arbitrary: Ys)
+  case 0
+  then have "Nt X # map Nt Xs = map Nt Ys"
+    by (smt (verit, best) list.inj_map_strong map_eq_Cons_conv relpowp.simps(1) sym.inject(1))
+  
+  with 0 have "[X] @ Xs = Ys \<and> P \<turnstile> [Nt X] \<Rightarrow>l* map Nt [X]"
+    by (smt (verit, ccfv_SIG) append_Cons append_Nil list.inj_map_strong list.simps(8) map_eq_Cons_conv rtranclp.rtrancl_refl sym.inject(1))
+  then show ?case
+    by auto
+next
+  case (Suc n)
+
+  then obtain z where "P \<turnstile> Nt X # map Nt Xs \<Rightarrow>l(n) z" and "P \<turnstile> z \<Rightarrow>l map Nt Ys"
+    by auto
+
+  from \<open>P \<turnstile> z \<Rightarrow>l map Nt Ys\<close> obtain xs' where "z = map Nt xs'"
+    using derivel_not_elim_tm by blast
+  with \<open>P \<turnstile> Nt X # map Nt Xs \<Rightarrow>l(n) z\<close> have "P \<turnstile> Nt X # map Nt Xs \<Rightarrow>l(n) map Nt xs'"
+    by simp
+  with Suc(1) assms(2) obtain Ys'1 where IH: "Ys'1 @ Xs = xs' \<and> P \<turnstile> [Nt X] \<Rightarrow>l(n) map Nt Ys'1"
+    by fast
+
+  from \<open>z = map Nt xs'\<close> \<open>P \<turnstile> z \<Rightarrow>l map Nt Ys\<close> have "P \<turnstile> map Nt xs' \<Rightarrow>l map Nt Ys"
+    by fast
+
+  show ?case
+  proof (cases xs')
+    case Nil
+    with \<open>P \<turnstile> map Nt xs' \<Rightarrow>l map Nt Ys\<close> have "P \<turnstile> [] \<Rightarrow>l map Nt Ys" by simp
+    then have False by simp
+    then show ?thesis by fast
+  next
+    case (Cons xs'1 xs's)
+    with \<open>P \<turnstile> map Nt xs' \<Rightarrow>l map Nt Ys\<close> have "P \<turnstile> Nt xs'1 # map Nt xs's \<Rightarrow>l map Nt Ys"
+      by simp
+    then obtain Ys'2 where step: "Ys'2 @ xs's = Ys" "P \<turnstile> [Nt xs'1] \<Rightarrow>l map Nt Ys'2"
+      using derivel_nts_suffix by fast
+    
+    show ?thesis
+    proof (cases "Ys'1")
+      case Nil
+      with IH Cons have "P \<turnstile> [Nt X] \<Rightarrow>l(n) map Nt []"
+        by auto
+      then have False using Eps_free_derivels_Nil
+        by (metis assms(2) list.discI map_is_Nil_conv relpowp_imp_rtranclp) 
+      then show ?thesis by (rule FalseE)
+    next
+      case innerCons: (Cons Ys'1_1 Ys'1s)
+      with IH Cons have "Ys'1_1 = xs'1"
+        by auto
+
+      with IH innerCons have IH_new: "xs'1 # Ys'1s @ Xs = xs' \<and> P \<turnstile> [Nt X] \<Rightarrow>l(n) Nt xs'1 # map Nt Ys'1s"
+        by simp
+      with Cons step(1) have "Ys'2 @ Ys'1s @ Xs = Ys"
+        by blast
+
+      moreover from IH_new \<open>P \<turnstile> [Nt xs'1] \<Rightarrow>l map Nt Ys'2\<close> have "P \<turnstile> [Nt X] \<Rightarrow>l(Suc n) map Nt Ys'2 @ map Nt Ys'1s"
+        using derivel_append by fastforce
+      then have "P \<turnstile> [Nt X] \<Rightarrow>l(Suc n) map Nt (Ys'2 @ Ys'1s)"
+        by simp 
+
+      ultimately show ?thesis
+        by auto
+    qed
+  qed
+qed
+
+
+
+
 
 
 (*  TODO: once, the core of the proof is done,
@@ -45,23 +273,22 @@ proof -
   fix G
 
   (* obtain a grammar for L G that is in CNF *)
-  have "\<forall>G::('n::infinite,'t) cfg. \<exists>G0::('n,'t) cfg. (cnf G0) \<and> (L G0 = L G - {[]})"
-    by (rule cnf_exists)
-  then obtain "G0" where cnf: "(cnf (G0::('n,'t) cfg))"
-                and cnf_L_eq: "(L G0 = L (G::('n::infinite,'t) cfg) - {[]})"
-    by auto
+  obtain G0 where G0_def: "G0 = some_cnf (G::('n::infinite,'t) cfg)" by fast
+  then have cnf: "(cnf (G0::('n,'t) cfg))"
+        and cnf_L_eq: "(L G0 = L (G::('n::infinite,'t) cfg) - {[]})"
+    using some_cnf_cnf by fast+
 
   (* witness function for G_A,a. The grammars adhere to G_props *)
-  obtain witness where func: "(\<And>A a. (\<exists>G. (witness:: 'n \<Rightarrow> 't \<Rightarrow> (nat,'n) cfg) A a = G \<and> G_props A a G G0))"
-    by (meson exists_rlin_G_for_R cnf)
+  obtain witness where witness: "(\<And>A a. (let G = (witness:: 'n \<Rightarrow> 't \<Rightarrow> (nat,'n) cfg) A a in G_props A a G0 G))"
+    by (meson exists_G_for_R cnf)
 
   (* Derive a witness function for G_A,a
      that renames the nonterminals to ensure that these are disjoint *)
   obtain renamed_wittness where renamed_wittness_def: "renamed_wittness = (\<lambda> A a. (rename_cfg (Renamed A a)) (witness A a))" by simp
   
   (* Grammars returned by renamed_wittness also adhere to G_props *)
-  then have "(\<And>A a. (\<exists>G. renamed_wittness A a = G \<and> G_props A a G G0))"
-    by (smt (verit) G_props_def cfg_rename_L cfg_rename_rlin2 func injI renamed.inject(2))
+  then have renamed_wittness_G_props: "(\<And>A a. (let G = renamed_wittness A a in G_props A a G0 G))"
+    by (smt (verit) G_props_def cfg_rename_L cfg_rename_rlin2 witness injI renamed.inject(2))
 
   (* The nonterminals of different grammars returned by renamed_wittness are disjoint.
      This fact is currently not yet used, but will later be relevant. *)
@@ -85,11 +312,12 @@ proof -
      The productions of G1 are the union of ?G1_new_prods with the productions of G0R *)
   obtain G0R where G0R_def: "(G0R::(('n,'t) renamed,'t) cfg) = rename_cfg Original G0" by fast
   obtain G_union where G_union_def: "(G_union::(('n,'t) renamed,'n) Prods) = 
-      (\<Union>A\<in>(nts (prods G0)). (\<Union> a\<in>(tms (prods G0)). set(prods (renamed_wittness A a))))"
+      (\<Union>A. (\<Union> a. set(prods (renamed_wittness A a))))"
     by fast
   let ?G1_new_prods = "map_tms_Prods Original G_union"
   let ?G0R_prods = "set (prods G0R)"
   let ?G1_prods = "?G0R_prods \<union> ?G1_new_prods"
+  (* TODO: skip G1 *)
 
   (* G0R is still in CNF *)
   from cnf have "cnf G0R" unfolding G0R_def by (rule cfg_rename_cnf_dir1)
@@ -167,186 +395,421 @@ proof -
   then have G1_prods_Original: "\<And>A w. (A,w) \<in> ?G1_prods \<Longrightarrow> (\<exists>nt. A = Original nt) \<Longrightarrow> (A,w) \<in> ?G0R_prods"
     unfolding Lhss_def by blast
 
-  (*
-    First part of the proof of equivalence of G1 and G2:
-      Show by induction on the length of the leftmost derivation, that for each
-      sequence of nonterminals (that originate from G0R), G1 and G2 produce the
-      same sequences of terminals.
-   *)
-  have "\<And>ss x. (?G1_prods \<turnstile> (map (Nt o Original) ss) \<Rightarrow>* (map Tm x)) \<Longrightarrow>
-                (?G2_prods \<turnstile> (map (Nt o Original) ss) \<Rightarrow>* (map Tm x))"
+
+
+  have G0R_deriveln_iff_G1:
+      "\<And>u n v. (?G0R_prods \<turnstile> map (Nt o Original) u \<Rightarrow>l(n) map Tm v) =
+                (?G1_prods \<turnstile> map (Nt o Original) u \<Rightarrow>l(n) map Tm v)"
+  proof -
+    fix u n v
+    note \<open>Nts ?G0R_prods \<inter> Lhss ?G1_new_prods = {}\<close>
+    moreover have "nts_of_syms (map (Nt o Original) u) \<inter> Lhss ?G1_new_prods = {}"
+      unfolding nts_of_syms_def Lhss_def using Lhss_def \<open>\<And>S. Original S \<notin> Lhss G_union\<close> by fastforce
+    ultimately show "(?G0R_prods \<turnstile> map (Nt o Original) u \<Rightarrow>l(n) map Tm v) =
+                     (?G1_prods \<turnstile> map (Nt o Original) u \<Rightarrow>l(n) map Tm v)"
+      using append_unreachable_productions_deriveln_iff by blast
+  qed
+
+  then have G0R_derivels_iff_G1:
+      "\<And>u v. (?G0R_prods \<turnstile> map (Nt o Original) u \<Rightarrow>l* map Tm v) =
+                (?G1_prods \<turnstile> map (Nt o Original) u \<Rightarrow>l* map Tm v)"
+    by (simp add: rtranclp_power)
+
+
+  (* first direction *)
+  have G1_G2: "\<And>ss x. (?G1_prods \<turnstile> (map (Nt o Original) ss) \<Rightarrow>* map Tm x) \<Longrightarrow>
+                      (?G2_prods \<turnstile> (map (Nt o Original) ss) \<Rightarrow>* map Tm x)"
   proof -
     fix ss x
-    have "(?G1_prods \<turnstile> (map (Nt o Original) ss) \<Rightarrow>* (map Tm x)) \<Longrightarrow>
-          (?G2_prods \<turnstile> (map (Nt o Original) ss) \<Rightarrow>* (map Tm x))"
-    proof -
-      let ?ntss = "map (Nt o Original) ss"
-      assume "(?G1_prods \<turnstile> ?ntss \<Rightarrow>* (map Tm x))"
-      (* there must be a leftmost derivation *)
-      from this(1) have "(?G1_prods \<turnstile> ?ntss \<Rightarrow>l* (map Tm x))" by (rule derives_tms_imp_derivels)
-      (* obtain the length of that derivation *)
-      then have "\<exists>n. (?G1_prods \<turnstile> ?ntss \<Rightarrow>l(n) (map Tm x))"
-        by (rule rtranclp_imp_relpowp)
-      then obtain n where "?G1_prods \<turnstile> ?ntss \<Rightarrow>l(n) (map Tm x)" by auto
+    assume assm: "(?G1_prods \<turnstile> (map (Nt o Original) ss) \<Rightarrow>* (map Tm x))"
+    let ?ntss = "map (Nt o Original) ss"
 
-      (* Beginning of the actual induction proof:
-         Shows: If there is a leftmost derivation in G1 of length \<le> n
-           from any sequence of nonterminals contained in G0R to the terminal word x
-           then there must also be a derivation in G2
-       *)
-      fix sss
-      have "\<And>m. ?G1_prods \<turnstile> map (Nt o Original) sss \<Rightarrow>l(m) (map Tm x) \<Longrightarrow> m \<le> n \<Longrightarrow> 
-                 ?G2_prods \<turnstile> map (Nt o Original) sss \<Rightarrow>* (map Tm x)"
-      proof (induction n arbitrary: sss)
-        case 0
-        (* trivial, since both sides of the derivation must be [] then *)
+    (* there must be a leftmost derivation *)
+    from assm have "(?G1_prods \<turnstile> ?ntss \<Rightarrow>l* (map Tm x))"
+      by (rule derives_tms_imp_derivels)
+
+    (* obtain the length of that derivation *)
+    then have "\<exists>n. (?G1_prods \<turnstile> ?ntss \<Rightarrow>l(n) (map Tm x))"
+      by (rule rtranclp_imp_relpowp)
+    then obtain n where "?G1_prods \<turnstile> ?ntss \<Rightarrow>l(n) (map Tm x)" by auto
+
+    (* unused
+
+    (* Beginning of the actual induction proof:
+       Shows: If there is a leftmost derivation in G1 of length \<le> n
+         from any sequence of nonterminals contained in G0R to the terminal word x
+         then there must also be a derivation in G2
+     *)
+    moreover have "?G1_prods \<turnstile> map (Nt o Original) ss \<Rightarrow>l* (map Tm x) \<Longrightarrow> 
+                   ?G2_prods \<turnstile> map (Nt o Original) ss \<Rightarrow>* (map Tm x)"
+    proof -
+      assume "?G1_prods \<turnstile> map (Nt o Original) ss \<Rightarrow>l* (map Tm x)"
+      then have "?G0R_prods \<turnstile> map (Nt o Original) ss \<Rightarrow>l* map Tm x"
+        using G0R_derivels_iff_G1 by fast
+
+      moreover note \<open>CNF ?G0R_prods\<close>
+      ultimately show "?G2_prods \<turnstile> map (Nt o Original) ss \<Rightarrow>* (map Tm x)"
+      proof (induction rule: cnf_derivels_induct)
+        case base
         then show ?case by simp
       next
-        case (Suc n)
+        case (step_nt_nt u A v B C)
+        then show ?case sorry 
+      next
+        case (step_tm u A v t)
+        then show ?case sorry  (* productions of this type are still contained *)
+      qed
+    qed
+
+    *)
+
+
+    (* Beginning of the actual induction proof:
+       Shows: If there is a leftmost derivation in G1 of length \<le> n
+         from any sequence of nonterminals contained in G0R to the terminal word x
+         then there must also be a derivation in G2
+     *)
+    moreover have "?G1_prods \<turnstile> map (Nt o Original) ss \<Rightarrow>l(n) (map Tm x) \<Longrightarrow> 
+                   ?G2_prods \<turnstile> map (Nt o Original) ss \<Rightarrow>* (map Tm x)"
+    proof (induction n arbitrary: ss x rule: nat_induct_leq)
+      case 0
+      (* trivial, since both sides of the derivation must be [] *)
+      then show ?case by simp
+    next
+      case (Leq n')
+      let ?ntsss = "map (Nt o Original) ss"
+      from Leq have in_G0R: "?G0R_prods \<turnstile> ?ntsss \<Rightarrow>l(Suc n') map Tm x"
+        using G0R_deriveln_iff_G1 by blast
+
+      show ?case
+      proof (cases "x = []")
+        (* There are no epsilon productions in CNF.
+           Thus, the empty word can only be derived if ss = [], in which case n would
+           have to be zero
+         *)
+        case True
+        with \<open>cnf G0R\<close> Leq(2) have "map (Nt \<circ> Original) ss = []"
+          using CNF_Eps_free Eps_free_derivels_Nil by (metis in_G0R list.map_disc_iff relpowp_imp_rtranclp)
+        with Leq have False
+          by auto
+        then show ?thesis by fast
+      next
+        case False
+        then obtain x1 xs where x1_xs: "x = x1 # xs"
+          by (meson neq_Nil_conv)
+        with \<open>?G0R_prods \<turnstile> ?ntsss \<Rightarrow>l(Suc n') map Tm x\<close> have "?G0R_prods \<turnstile> ?ntsss \<Rightarrow>l(Suc n') Tm x1 # map Tm xs"
+          by simp
+        then have "?G0R_prods \<turnstile> map Nt (map Original ss) \<Rightarrow>l(Suc n') Tm x1 # map Tm xs"
+          by simp
+
+        moreover note \<open>CNF ?G0R_prods\<close>
+        ultimately obtain T ns n1 n2 where
+           step1: "?G0R_prods \<turnstile> map Nt (map Original ss) \<Rightarrow>l(n1) Nt T # map Nt ns" and
+           step2: "?G0R_prods \<turnstile> Nt T # map Nt ns \<Rightarrow>l Tm x1 # map Nt ns" and
+           step3: "?G0R_prods \<turnstile> Tm x1 # map Nt ns \<Rightarrow>l(n2) Tm x1 # map Tm xs" and
+           sum: "n1 + 1 + n2 = Suc n'" using 
+              CNF_derivln_first_tm_strong[where 
+                      P="?G0R_prods"
+                  and u="(map Original ss)"
+                  and n="Suc n'"
+                  and t="x1"
+                  and v="map Tm xs"]
+          by blast
+
+        then obtain T' where T': "T = Original T'"
+          (* provable since T is a result of a derivation in ?G0R_prods starting from Original nonterminals*)
+          sorry
+
+        then obtain ns' where ns': "ns = map Original ns'"
+          (* provable since ns is a result of a derivation in ?G0R_prods starting from Original nonterminals*)
+          sorry
+
+
+        have "?G2_prods \<turnstile>map (Nt \<circ> Original) ss \<Rightarrow>* Tm x1 # map (Nt \<circ> Original) ns'"
+        proof (cases n1)
+          case 0
 
         (*
-          Proof idea for this case:
-            Due to lemma append_unreachable_productions_derive
-            sequences of derivations in G1 starting from original nonterminals can never
-            lead to sentinential words containing nonterminals that only G2 contains.
-            
-            Thus, if there is a leftmost derivation in G1, then the same derivation also is
-            possible in G0.
-            We can obtain such a derivation and then obtain the first step where
-            a terminal is introduced at the left end.
-              For that there is lemma CNF_derivln_first_tm_strong
+          from step2 have "(T, [Tm x1]) \<in> ?G0R_prods"
+            by (smt (verit, best) Cons_eq_append_conv append_self_conv2 derivel.simps list.inject not_Cons_self2 sym.distinct(1) sym.inject(1))
+        *)
 
-            Due to the construction, when the first terminal a is introduced,
-            also the start symbol S_A,a is generated. 
-            This is the first time, the derivations in G1 and G2 are different.
-              
-
-            Thus, the sentinential from in the G1 derivation has the following form:
-              Tm a # [Nt A] @ map Nt nts
-            And in G2:
-              Tm a # Nt (start (renamed_wittness A a)) @ map Nt nts
-                note: `(start (renamed_wittness A a))` the expression for `S_A,a`
-              
-            We know, that for all derivations
-              G1_prods \<turnstile> [Nt A] \<Rightarrow> y
-            which lead to terminals, there is a corresponding derivation G2 \<turnstile> [S_A,a] \<Rightarrow> y,
-            due to the construction.
-
-            Due to the induction hypothesis, we know
-              G1_prods \<turnstile> [map Nt nts] \<Rightarrow>* nts' \<Longrightarrow> G2_prods \<turnstile> [map Nt nts] \<Rightarrow>* nts'
-
-
-            It may be required to generalize the induction, so that not only (map Tm x) are derived,
-            but sequences of (at least one) terminals followed by nonterminals
-         *)
-
-
-
-
-        (* Most part of the remaining part of the "proof" is leftover from a previous,
-           failed attempt. Nevertheless, some facts may be helpful.
-         *)
-(*
-        from this(2) have "?G0R_prods \<union> ?G1_new_prods \<turnstile> map (Nt \<circ> Original) sss \<Rightarrow>l(m) map Tm x" by force
-        then have "?G0R_prods \<union> ?G1_new_prods \<turnstile> map (Nt \<circ> Original) sss \<Rightarrow>l* map Tm x"
-          by (simp add: relpowp_imp_rtranclp)
-        then have "?G0R_prods \<union> ?G1_new_prods \<turnstile> map (Nt \<circ> Original) sss \<Rightarrow>* map Tm x"
-          by (simp add: derivels_iff_derives)
-        moreover note \<open>Nts ?G0R_prods \<inter> Lhss ?G1_new_prods = {}\<close>
+          have "(T, [Tm x1]) \<in> ?G0R_prods"
+          proof -
+            from step2 have "(\<exists>(A, w)\<in>?G0R_prods. \<exists>u1 u2. 
+                Nt T # map Nt ns = map Tm u1 @ Nt A # u2 \<and> 
+                Tm x1 # map Nt ns = map Tm u1 @ w @ u2)"
+              by (simp only: derivel_iff)
+            then obtain A w u1 u2 where
+                   A_w: "(A, w)\<in>?G0R_prods"
+                and xs: "Nt T # map Nt ns = map Tm u1 @ Nt A # u2"
+                and ys: "Tm x1 # map Nt ns = map Tm u1 @ w @ u2"
+              by fast
   
-        from \<open>?G0R_prods \<union> ?G1_new_prods \<turnstile> map (Nt \<circ> Original) sss \<Rightarrow>* map Tm x\<close> 
-        have "nts_of_syms (map (Nt \<circ> Original) sss) \<subseteq> Nts (?G0R_prods \<union> ?G1_new_prods)"
-          by (metis derive_map_Tm_nts_in_prod_invariant list.map_comp nts_of_syms_map_Nt)
-        then have "nts_of_syms (map (Nt \<circ> Original) sss) \<subseteq> Lhss (?G0R_prods)"
-          unfolding nts_of_syms_def sorry
-        moreover have "nts_of_syms (map (Nt \<circ> Original) sss) = set (map (Original) sss)"
-          using nts_of_syms_map_Nt by (metis list.map_comp)
-  
-        ultimately have "nts_of_syms (map (Nt \<circ> Original) sss) \<subseteq> Nts (?G0R_prods)"
-          by simp
-  
-        ultimately have "nts_of_syms (map Tm x) \<subseteq> Nts ?G0R_prods"
-          using append_unreachable_productions_derive by blast 
-  
-        with Suc show ?case
-        proof (cases m)
-          case 0
-          with Suc show ?thesis by simp
-        next
-          let ?ntsss = "map (Nt o Original) sss"
-          case innerSuc: (Suc mn)
-          with Suc(2) have "?G1_prods \<turnstile> ?ntsss \<Rightarrow>l(Suc mn) map Tm x"
-            by blast
-  
-          thm CNF_derivln_first_tm_strong
-  
-  
-          then have "\<exists>y. (?G1_prods \<turnstile> ?ntsss \<Rightarrow>l y \<and> ?G1_prods \<turnstile> y \<Rightarrow>l(mn) (map Tm x))"
-            by (rule relpowp_Suc_D2)
-          then obtain y where "?G1_prods \<turnstile> ?ntsss \<Rightarrow>l y" and first_g1: "?G1_prods \<turnstile> y \<Rightarrow>l(mn) (map Tm x)" by auto
-  
-  
-          from first_g1 innerSuc Suc have first: "?G2_prods \<turnstile> y \<Rightarrow>* map Tm x" by auto
-  
-  
-          note \<open>?G1_prods \<turnstile> ss \<Rightarrow>l y\<close>
-          then have "(\<exists> (A,w) \<in> ?G1_prods. \<exists>u1 u2. ss = map Tm u1 @ Nt A # u2 \<and> y = map Tm u1 @ w @ u2)"
-            using derivel_iff
-            by blast 
-          then obtain A w u1 u2 where "(A,w) \<in> ?G1_prods" and ss: "ss = map Tm u1 @ Nt A # u2" and y: "y = map Tm u1 @ w @ u2" by auto
-  
-          have "?G2_prods \<turnstile> [Nt A] @ u2 \<Rightarrow>* w @ u2"
-          proof (cases A)
-            case (Original nt)
-            with \<open>(A,w) \<in> ?G1_prods\<close> have "(A,w) \<in> ?G0R_prods" using G1_prods_Original by auto
-            with \<open>CNF ?G0R_prods\<close> have "(\<exists>B C. w = [Nt B, Nt C]) \<or> (\<exists>t. w = [Tm t])"
-              unfolding CNF_def by fast
-            then show ?thesis
-            proof (elim disjE)
-              assume "(\<exists>B C. w = [Nt B, Nt C])"
-              then obtain B C where "w = [Nt B, Nt C]" by auto
-              show ?thesis sorry
-            next
-              assume "(\<exists>t. w = [Tm t])"
-              then obtain t where "w = [Tm t]" by auto
-              then have "\<not> removed_from_G2 (A,w)"
-                by (simp add: removed_from_G2_def)
-              then have "(A,w) \<in> G2_retained_prods"
-                unfolding G2_retained_prods_def removed_from_G2_def
-                using \<open>(A, w) \<in> ?G1_prods\<close> G1_prods_def by blast
-              then have "(A,w) \<in> ?G2_prods" unfolding ?G2_prods_def by simp
-              then have "?G2_prods \<turnstile> [Nt A] \<Rightarrow> w"
-                using derive_singleton by blast
-              then have "?G2_prods \<turnstile> [Nt A] @ u2 \<Rightarrow> w @ u2"
-                using derive_append_decomp by blast
-              then show ?thesis by simp
-            qed
-  
-            (* TODO: case distinction between different possible cases of w *)
-  
-          next
-            (* due to \<open>original ss\<close>, this is case not possible *)
-            case (Renamed AA aa num)
-            with ss Suc(4) show ?thesis unfolding original_sym_def by auto
+            (* TODO: this is a pattern used more often, it could be refactored into its own lemma *)
+            then have u1: "u1 = []"
+              by (metis Nil_is_map_conv hd_append list.sel(1) sym.simps(4))
+            with xs have "T = A"
+              by auto
+            from xs u1 have "map Nt ns = u2"
+              by simp
+            with u1 ys have "w = [Tm x1]"
+              by simp
+            from A_w \<open>T = A\<close> \<open>w = [Tm x1]\<close> show "(T, [Tm x1]) \<in> ?G0R_prods"
+              by blast
           qed
-          then have "?G2_prods \<turnstile> Nt A # u2 \<Rightarrow>* w @ u2"
-            by (metis append.left_neutral append_Cons derives_append)
-          then have "?G2_prods \<turnstile> map Tm u1 @ Nt A # u2 \<Rightarrow>* map Tm u1 @ w @ u2"
-            using derives_prepend by blast 
-          with ss y have second: "?G2_prods \<turnstile> ss \<Rightarrow>* y" by simp
-  
-          from first second show ?thesis by auto
-        qed
-      qed
-      moreover note original
-      ultimately show "?G2_prods \<turnstile> ss \<Rightarrow>* map Tm x" by simp
-*)
+          then have "(T, [Tm x1]) \<in> ?G1_prods"
+            by blast
+          then have "(T, [Tm x1]) \<in> G2_retained_prods"
+            unfolding G2_retained_prods_def removed_from_G2_def by simp
+          then have "(T, [Tm x1]) \<in> ?G2_prods"
+            by blast
+          then have "?G2_prods \<turnstile> Nt T # map Nt ns \<Rightarrow>l Tm x1 # map Nt ns"
+            by (simp add: derivel_Nt_Cons)
 
+          moreover from 0 step1 have "set (prods G0R) \<turnstile> map Nt (map Original ss) \<Rightarrow>l(0) Nt T # map Nt ns"
+            by blast
+          then have "map Nt (map Original ss) = Nt T # map Nt ns"
+            using relpowp_0_E by (smt (verit, best) Cons_eq_map_conv list.inj_map_strong sym.inject(1)) 
+        
+          then show ?thesis
+            by (metis calculation derivels_imp_derives map_map ns' r_into_rtranclp)
+        next
+          case (Suc n1')
+          with step1 have "?G0R_prods \<turnstile> map Nt (map Original ss) \<Rightarrow>l(Suc n1') Nt T # map Nt ns" by simp
+          then obtain middle where 
+                    step1A: "?G0R_prods \<turnstile> map Nt (map Original ss) \<Rightarrow>l middle"
+                and step1B: "?G0R_prods \<turnstile> middle \<Rightarrow>l(n1') Nt T # map Nt ns"
+            using relpowp_Suc_E2 by metis
+
+          then obtain middle_nts where middle_nts: "middle = map Nt middle_nts"
+            by (metis deriveln_not_elim_tm list.simps(9))
+
+          with step1B have middle_nts_not_Nil: "middle_nts \<noteq> []"
+            by auto
+
+          with step1A have "ss \<noteq> []"
+            by auto
+
+          from middle_nts_not_Nil obtain middle_nts1 middle_ntss where middle_nts1: "middle_nts = middle_nts1 # middle_ntss"
+            using list.exhaust_sel by blast
+
+          with middle_nts step1B have "?G0R_prods \<turnstile> Nt middle_nts1 # map Nt middle_ntss \<Rightarrow>l(n1') map Nt (T # ns)"
+            by simp
+
+          moreover from \<open>CNF ?G0R_prods\<close> have "Eps_free ?G0R_prods"
+            by (rule CNF_Eps_free)
+
+          ultimately obtain Ys' where Ys': "Ys' @ middle_ntss = T # ns \<and> ?G0R_prods \<turnstile> [Nt middle_nts1] \<Rightarrow>l(n1') map Nt Ys'"
+            using deriveln_nts_suffix by fast
+  
+          then have "Ys' \<noteq> []"
+            (* TODO: make nicer *)
+            by (metis Eps_free_derivels_Nil \<open>Eps_free (set (prods G0R))\<close> length_0_conv length_map not_Cons_self2 relpowp_imp_rtranclp)
+
+          with Ys' obtain Ys's where Ys's: "Ys' = T # Ys's"
+            by (meson append_eq_Cons_conv)
+
+          with Ys' have "?G0R_prods \<turnstile> [Nt middle_nts1] \<Rightarrow>l(n1') map Nt (T # Ys's)"
+            by blast
+          then have "?G0R_prods \<turnstile> [Nt middle_nts1] \<Rightarrow>l(n1') Nt T # map Nt (Ys's)"
+            by simp
+
+          moreover from step2 have "(T, [Tm x1]) \<in> ?G0R_prods"
+            by (simp add: derivel_Nt_Cons)
+          then have "?G0R_prods \<turnstile> Nt T # map Nt Ys's \<Rightarrow>l Tm x1 # map Nt Ys's"
+            by (simp add: derivel_Nt_Cons)
+          ultimately have "?G0R_prods \<turnstile> [Nt middle_nts1] \<Rightarrow>l(Suc n1') Tm x1 # map Nt (Ys's)"
+            by auto
+          then have "?G0R_prods \<turnstile> [Nt middle_nts1] \<Rightarrow>l* Tm x1 # map Nt (Ys's)"
+            by (rule relpowp_imp_rtranclp)
+
+          obtain Ys's' where Ys's': "Ys's = map Original Ys's'"
+            sorry (* provable since ?G0R_prods only contains original nonterminals *)
+
+          from middle_nts step1A have "\<exists>middle_nts'. middle_nts = map Original middle_nts'"
+            sorry (* provable since ?G0R_prods only contains original nonterminals *)
+
+          then obtain middle_nts1' where middle_nts1': "middle_nts1 = Original middle_nts1'"
+            using middle_nts1 by blast
+
+          with \<open>?G0R_prods \<turnstile> [Nt middle_nts1] \<Rightarrow>l* Tm x1 # map Nt (Ys's)\<close> Ys's'
+          have "?G0R_prods \<turnstile> [Nt (Original middle_nts1')] \<Rightarrow>l* Tm x1 # map Nt (map Original Ys's')"
+            by simp
+          then have "?G0R_prods \<turnstile> rename_syms Original [Nt middle_nts1'] \<Rightarrow>l* Tm x1 # map Nt (map Original Ys's')"
+            by simp
+          then have "?G0R_prods \<turnstile> rename_syms Original [Nt middle_nts1'] \<Rightarrow>l* Tm x1 # rename_syms Original (map Nt Ys's')"
+            by (simp only: map_rename_syms)
+          then have "?G0R_prods \<turnstile> rename_syms Original [Nt middle_nts1'] \<Rightarrow>l* rename_syms Original (Tm x1 # map Nt Ys's')"
+            by simp
+          then have "set (rename_prods Original (prods (G0)))
+                      \<turnstile> rename_syms Original [Nt middle_nts1']
+                      \<Rightarrow>l* rename_syms Original (Tm x1 # map Nt Ys's')"
+            unfolding G0R_def
+            by (metis cfg_rename_derivels_iff inj_Original prods_rename_cfg_rename_prods)
+
+          then have "set (prods (G0)) \<turnstile> [Nt middle_nts1'] \<Rightarrow>l* (Tm x1 # map Nt Ys's')"
+            using cfg_rename_derivels_iff inj_Original
+            by blast
+
+          then have "Ys's' \<in> R_func (set (prods G0)) middle_nts1' x1"
+            unfolding R_func_def by blast
+          moreover have "G_props middle_nts1' x1 G0 (renamed_wittness middle_nts1' x1)"
+            using renamed_wittness_G_props by auto
+          ultimately have "set (prods (renamed_wittness middle_nts1' x1))
+                            \<turnstile> [Nt (start (renamed_wittness middle_nts1' x1))]
+                            \<Rightarrow>* map Tm Ys's'"
+            unfolding R_func_def G_props_def Lang_def by auto
+
+          then have "G_union \<turnstile> [Nt (start (renamed_wittness middle_nts1' x1))] \<Rightarrow>* map Tm Ys's'"
+            unfolding G_union_def by (smt (verit, ccfv_threshold) UnionI image_iff iso_tuple_UNIV_I psubRtcDeriv)
+
+          then have "?G1_new_prods \<turnstile> [Nt (start (renamed_wittness middle_nts1' x1))] \<Rightarrow>* map Nt (map Original Ys's')"
+            using map_tms_Prods_derivel[where P=G_union
+                                          and a="[start (renamed_wittness middle_nts1' x1)]"
+                                          and b="Ys's'"
+                                          and f=Original]
+            by simp
+
+          then have "?G1_prods \<turnstile> [Nt (start (renamed_wittness middle_nts1' x1))] \<Rightarrow>* map Nt (map Original Ys's')"
+            by (metis Un_iff psubRtcDeriv)
+
+          then have "G2_retained_prods \<turnstile> [Nt (start (renamed_wittness middle_nts1' x1))] \<Rightarrow>* map Nt (map Original Ys's')"
+            sorry (*  no production used for this derivation has an Original nonterminal on its left hand side
+                      \<rightarrow> thus none of these productions has been removed
+                      rather difficult to prove, probably it is easier to not use define a G1 at all
+                   *)
+
+          then have "?G2_prods \<turnstile> [Nt (start (renamed_wittness middle_nts1' x1))] \<Rightarrow>* map Nt (map Original Ys's')"
+            by (metis Un_iff psubRtcDeriv)
+
+
+
+
+          from step1A middle_nts middle_nts1 have "?G0R_prods \<turnstile> map Nt (map Original ss) \<Rightarrow>l Nt middle_nts1 # map Nt middle_ntss"
+            by simp
+
+          moreover from this have "ss \<noteq> []"
+            by auto
+          then obtain ss1 sss where "ss = ss1 # sss"
+            by (meson list.exhaust)
+
+          ultimately have "?G0R_prods \<turnstile> Nt (Original ss1) # map Nt (map Original sss) \<Rightarrow>l Nt middle_nts1 # map Nt middle_ntss"
+            by simp
+          then have "?G0R_prods \<turnstile> Nt (Original ss1) # map Nt (map Original sss) \<Rightarrow>l map Nt (middle_nts1 # middle_ntss)"
+            by simp
+
+          then obtain prefix where "prefix @ map Original sss = middle_nts1 # middle_ntss"
+                                   "?G0R_prods \<turnstile> [Nt (Original ss1)] \<Rightarrow>l map Nt prefix"
+            using derivel_nts_suffix by fast
+          then have "(Original ss1, map Nt prefix) \<in> ?G0R_prods"
+            by (simp add: derivel_Nt_Cons)
+
+          note \<open>?G0R_prods \<turnstile> Nt (Original ss1) # map Nt (map Original sss) \<Rightarrow>l map Nt (middle_nts1 # middle_ntss)\<close>
+          then obtain middle_ntss1 middle_ntsss
+            where "middle_ntss = middle_ntss1 # middle_ntsss"
+              and "[Original middle_nts1', middle_ntss1] = prefix"
+            sorry (* can be obtained due to CNF *)
+
+          with \<open>(Original ss1, map Nt prefix) \<in> ?G0R_prods\<close> have "(Original ss1, [Nt (Original middle_nts1'), Nt middle_ntss1]) \<in> ?G1_prods"
+            by auto
+
+          then have "(Original ss1, [Tm x1, Nt (start (renamed_wittness middle_nts1' x1)), Nt middle_ntss1]) \<in> G2_new_prods"
+            unfolding G2_new_prods_def by blast
+
+          then have "?G2_prods \<turnstile> Nt (Original ss1) # map Nt (map Original sss)
+                                  \<Rightarrow>* [Tm x1, Nt (start (renamed_wittness middle_nts1' x1)), Nt middle_ntss1] @ map Nt (map Original sss)"
+            by (simp add: derivel_Nt_Cons derivel_imp_derive r_into_rtranclp)
+
+          moreover from \<open>?G2_prods \<turnstile> [Nt (start (renamed_wittness middle_nts1' x1))] \<Rightarrow>* map Nt (map Original Ys's')\<close>
+          have "?G2_prods \<turnstile> [Tm x1, Nt (start (renamed_wittness middle_nts1' x1))] \<Rightarrow>* Tm x1 # map Nt (map Original Ys's')"
+            by (rule derives_Cons)
+          then have "?G2_prods \<turnstile> [Tm x1, Nt (start (renamed_wittness middle_nts1' x1)), Nt middle_ntss1] \<Rightarrow>* Tm x1 # map Nt ((map Original Ys's')) @ [Nt middle_ntss1]"
+            by (metis append.left_neutral append_Cons derives_append)
+          then have "?G2_prods \<turnstile> [Tm x1, Nt (start (renamed_wittness middle_nts1' x1)), Nt middle_ntss1] @ map Nt (map Original sss) \<Rightarrow>* Tm x1 # map Nt ((map Original Ys's')) @ [Nt middle_ntss1] @ map Nt (map Original sss)"
+             by (metis Cons_eq_appendI append_assoc derives_append)
+
+          ultimately have "?G2_prods \<turnstile> Nt (Original ss1) # map Nt (map Original sss)
+                                  \<Rightarrow>* Tm x1 # map Nt (map Original Ys's') @ Nt middle_ntss1 # map Nt (map Original sss)"
+            by simp 
+
+          with Ys's' have "?G2_prods \<turnstile> Nt (Original ss1) # map Nt (map Original sss)
+                                  \<Rightarrow>* Tm x1 # map Nt Ys's @ Nt middle_ntss1 # map Nt (map Original sss)"
+            by simp
+          then have "?G2_prods \<turnstile> Nt (Original ss1) # map Nt (map Original sss)
+                                  \<Rightarrow>* Tm x1 # map Nt (Ys's @ middle_ntss1 # map Original sss)"
+            by simp
+          with \<open>ss = ss1 # sss\<close> have "?G2_prods \<turnstile> map Nt (map Original ss)
+                                  \<Rightarrow>* Tm x1 # map Nt (Ys's @ middle_ntss1 # map Original sss)"
+            by simp
+
+          moreover have "Ys's @ middle_ntss1 # (map Original sss) = map Original ns'"
+            using Ys' Ys's \<open>[Original middle_nts1', middle_ntss1] = prefix\<close> \<open>prefix @ map Original sss = middle_nts1 # middle_ntss\<close> ns' by force
+          ultimately have "?G2_prods \<turnstile> map (Nt \<circ> Original) ss \<Rightarrow>* Tm x1 # map Nt (map Original ns')"
+            by simp
+          then have "?G2_prods \<turnstile> map (Nt \<circ> Original) ss \<Rightarrow>* Tm x1 # map (Nt \<circ> Original) ns'"
+            by simp
+          then show ?thesis by simp
+        qed
+
+        moreover have "?G2_prods \<turnstile> Tm x1 # map (Nt \<circ> Original) ns' \<Rightarrow>* map Tm x"
+        proof -
+          from step3 have "?G0R_prods \<turnstile> map Nt ns \<Rightarrow>l(n2) map Tm xs"
+            by (simp add: deriveln_Tm_Cons)
+          with \<open>ns = map Original ns'\<close> have "?G0R_prods \<turnstile> map (Nt o Original) ns' \<Rightarrow>l(n2) map Tm xs"
+            by simp
+          then have  "?G1_prods \<turnstile> map (Nt o Original) ns' \<Rightarrow>l(n2) map Tm xs"
+            using G0R_deriveln_iff_G1 by blast
+          moreover from sum have "n2 \<le> n'" by auto
+          moreover note Leq.IH
+          ultimately have "?G2_prods \<turnstile> map (Nt \<circ> Original) ns' \<Rightarrow>* map Tm xs"
+            by fast
+          then have "?G2_prods \<turnstile> Tm x1 # map (Nt \<circ> Original) ns' \<Rightarrow>* Tm x1 # map Tm xs"
+            by (rule derives_Cons)
+          then show "?G2_prods \<turnstile> Tm x1 # map (Nt \<circ> Original) ns' \<Rightarrow>* map Tm x"
+            using x1_xs by simp
+        qed
+
+        ultimately show ?thesis
+          by (rule rtranclp_trans)
+      qed
+    qed
+
+    ultimately show "(?G2_prods \<turnstile> (map (Nt o Original) ss) \<Rightarrow>* (map Tm x))" by fast
+  qed
+
+
+  (* second direction *)
+  have G2_G1: "\<And>ss x. (?G2_prods \<turnstile> (map (Nt o Original) ss) \<Rightarrow>* (map Tm x)) \<Longrightarrow>
+                (?G1_prods \<turnstile> (map (Nt o Original) ss) \<Rightarrow>* (map Tm x))"
+    sorry
+
+  
+
+  have "Lang ?G1_prods (Original (start G0)) = Lang ?G2_prods (Original (start G0))"
+    unfolding Lang_def apply(rule Collect_eqI)
+  proof
+    fix x
+    assume "?G1_prods \<turnstile> [Nt (Original (start G0))] \<Rightarrow>* map Tm x"
+    then show "?G2_prods \<turnstile> [Nt (Original (start G0))] \<Rightarrow>* map Tm x"
+      using G1_G2
+      by (metis (no_types, lifting) Nil_is_map_conv comp_apply list.simps(9)) 
+  next
+    fix x
+    assume "?G2_prods \<turnstile> [Nt (Original (start G0))] \<Rightarrow>* map Tm x"
+    then show "?G1_prods \<turnstile> [Nt (Original (start G0))] \<Rightarrow>* map Tm x" 
+      using G2_G1
+      by (metis (no_types, lifting) Nil_is_map_conv comp_apply list.simps(9)) 
+  qed
+
+
+  (* G2 is not yet in GNF, since it can contain epsilon-productions *)
+  (* TODO: prove, that eliminating epsilon-productions does not yield unit productions *)
 
   show ?thesis sorry
 qed
 
 
-
+lemma "(x = y) \<Longrightarrow> (\<And>e. ((e \<in> x) \<longleftrightarrow> (e \<in> y)))"  using [[simp_trace]] by simp
 
 end
