Gschossmann/cfg_merging.thy
@@ -6,84 +6,356 @@ begin
   This theory provides lemmas relevant when combining
   the productions of two grammars with disjoint
   sets of nonterminals.
-
-  The theory is nearly complete: I could not prove one fact that seems
-  to be identical to another, already proven fact at first, but is
-  actually different in some subtle that the display does not show. 
 *)
+
+
+
+
+(* helper for deriven_nts_prods_subset *)
+lemma derivel_nts_prods_subset:
+  assumes "P \<turnstile> u \<Rightarrow>l v"
+  shows "nts_of_syms v \<subseteq> Nts P \<union> nts_of_syms u"
+proof
+  fix x
+  assume asm: "x \<in> nts_of_syms v"
+
+  from assms(1) have "(\<exists>(A, w)\<in>P. \<exists>u1 u2. u = map Tm u1 @ Nt A # u2 \<and> v = map Tm u1 @ w @ u2)"
+    by (simp only: derivel_iff)
+  then obtain A w u1 u2
+      where "(A,w) \<in> P"
+        and u: "u = map Tm u1 @ Nt A # u2"
+        and v: "v = map Tm u1 @ w @ u2"
+    by fast
+
+  then show "x \<in> Nts P \<union> nts_of_syms u"
+  proof (cases "x \<in> nts_of_syms w")
+    case True
+    with \<open>(A, w) \<in> P\<close> show ?thesis unfolding Nts_def by auto
+  next
+    case False
+    with asm v have "x \<in> nts_of_syms (map Tm u1 @ u2)"
+      by simp
+    with u have "x \<in> nts_of_syms u" unfolding nts_of_syms_def by simp
+    then show "x \<in> Nts P \<union> nts_of_syms u" by simp
+  qed
+qed
+
+
+
+(* helper for deriven_nts_prods_subset *)
+lemma derive_nts_prods_subset:
+  assumes "P \<turnstile> u \<Rightarrow> v"
+  shows "nts_of_syms v \<subseteq> Nts P \<union> nts_of_syms u"
+proof
+  fix x
+  assume asm: "x \<in> nts_of_syms v"
+
+  from assms(1) have "(\<exists>(A, w)\<in>P. \<exists>u1 u2. u = u1 @ Nt A # u2 \<and> v = u1 @ w @ u2)"
+    by (simp only: derive_iff)
+  then obtain A w u1 u2
+      where "(A,w) \<in> P"
+        and u: "u = u1 @ Nt A # u2"
+        and v: "v = u1 @ w @ u2"
+    by fast
+
+  then show "x \<in> Nts P \<union> nts_of_syms u"
+  proof (cases "x \<in> nts_of_syms w")
+    case True
+    with \<open>(A, w) \<in> P\<close> show ?thesis unfolding Nts_def by auto
+  next
+    case False
+    with asm v have "x \<in> nts_of_syms (u1 @ u2)"
+      by simp
+    with u have "x \<in> nts_of_syms u" unfolding nts_of_syms_def by simp
+    then show "x \<in> Nts P \<union> nts_of_syms u" by simp
+  qed
+qed
 
 
 (* any derived word can only contain nonterminals that are part of
    either part of the grammar's nonterminals or contained in the
    word it is derived from *)
-lemma nts_prods_subset:
-  assumes deriv: "P \<turnstile> u \<Rightarrow>* v"
+lemma deriveln_nts_prods_subset:
+  assumes deriv: "P \<turnstile> u \<Rightarrow>l(n) v"
   shows "nts_of_syms v \<subseteq> Nts P \<union> nts_of_syms u"
-proof
-  fix x
-  assume asm: "x \<in> nts_of_syms v"
-  show "x \<in> Nts P \<union> nts_of_syms u"
-  proof
-    assume "x \<notin> nts_of_syms u"
-    from deriv this show "x \<in> Nts P"
-    proof (induction rule: derives_induct')
-      case base
-      with asm show ?case by simp
-    next
-      case (step pre A post a)
-      then show ?case
-      proof (cases "x \<in> nts_of_syms a")
-        case True
-        with \<open>(A, a) \<in> P\<close> show ?thesis unfolding Nts_def by auto
-      next
-        case False
-        with step(4) have "x \<notin> nts_of_syms (pre @ post)"
-          by (metis UnCI UnE nts_of_syms_append)
-        with False have  "x \<notin> nts_of_syms (pre @ a @ post)"
-          by simp
-        with step(3) show "x \<in> Nts P" by simp
-      qed
+proof -
+  from assms show ?thesis
+  proof (induction n arbitrary: v)
+    case 0
+    then show ?case by simp
+  next
+    case (Suc n)
+    then obtain v' where parts: "P \<turnstile> u \<Rightarrow>l(n) v' \<and> P \<turnstile> v' \<Rightarrow>l v"
+      by (meson relpowp_Suc_E)
+    with Suc have "nts_of_syms v' \<subseteq> Nts P \<union> nts_of_syms u" by fast
+    moreover from parts have "nts_of_syms v \<subseteq> Nts P \<union> nts_of_syms v'"
+      using derivel_nts_prods_subset by blast
+    ultimately show "nts_of_syms v \<subseteq> Nts P \<union> nts_of_syms u" by fast 
+  qed
+qed
+
+
+
+(* any derived word can only contain nonterminals that are part of
+   either part of the grammar's nonterminals or contained in the
+   word it is derived from *)
+lemma deriven_nts_prods_subset:
+  assumes deriv: "P \<turnstile> u \<Rightarrow>(n) v"
+  shows "nts_of_syms v \<subseteq> Nts P \<union> nts_of_syms u"
+proof -
+  from assms show ?thesis
+  proof (induction n arbitrary: v)
+    case 0
+    then show ?case by simp
+  next
+    case (Suc n)
+    then obtain v' where parts: "P \<turnstile> u \<Rightarrow>(n) v' \<and> P \<turnstile> v' \<Rightarrow> v"
+      by (meson relpowp_Suc_E)
+    with Suc have "nts_of_syms v' \<subseteq> Nts P \<union> nts_of_syms u" by fast
+    moreover from parts have "nts_of_syms v \<subseteq> Nts P \<union> nts_of_syms v'"
+      using derive_nts_prods_subset by blast
+    ultimately show "nts_of_syms v \<subseteq> Nts P \<union> nts_of_syms u" by fast 
+  qed
+qed
+
+
+
+
+
+
+
+
+
+
+
+(* helper for append_unreachable_productions_derivels *)
+lemma append_unreachable_productions_derivel:
+  assumes "old \<union> new \<turnstile> u \<Rightarrow>l v"
+      and "Nts old \<inter> Lhss new = {}"
+      and "nts_of_syms u \<inter> Lhss new = {}"
+    shows "old \<turnstile> u \<Rightarrow>l v \<and> nts_of_syms v \<inter> Lhss new = {}"
+proof -
+  thm derivel_iff
+  from assms(1) have "(\<exists>(A, w)\<in>(old \<union> new). \<exists>u1 u2. u = map Tm u1 @ Nt A # u2 \<and> v = map Tm u1 @ w @ u2)"
+    by (simp only: derivel_iff)
+  then obtain A w u' v' where
+        A_w: "(A, w)\<in>(old \<union> new)"
+      and u: "u = map Tm u' @ Nt A # v'"
+      and v: "v = map Tm u' @ w @ v'"
+    by fast
+  then have "(A,w) \<in> old \<or> (A,w) \<in> new" by simp
+  then show ?thesis
+  proof (elim disjE)
+    assume "(A, w) \<in> old"
+    with u v have "(A, w) \<in> old"
+        and u: "u = map Tm u' @ Nt A # v'"
+        and v: "v = map Tm u' @ w @ v'" by auto
+    then have "old \<turnstile> u \<Rightarrow>l v" using derivel.intros by fastforce
+    moreover have "nts_of_syms v \<inter> Lhss new = {}"
+    proof -
+      from v have "nts_of_syms v = nts_of_syms (map Tm u') \<union> nts_of_syms w \<union> nts_of_syms v'"
+        unfolding nts_of_syms_def by auto
+      moreover from \<open>(A, w) \<in> old\<close> have "nts_of_syms w \<subseteq> Nts old"
+        unfolding nts_of_syms_def Nts_def by auto
+      with assms have "nts_of_syms w \<inter> Lhss new = {}"
+        by fast
+      moreover from u assms have "nts_of_syms (map Tm u') \<inter> Lhss new = {}"
+        by auto
+      moreover from u assms have "nts_of_syms v' \<inter> Lhss new = {}"
+        unfolding nts_of_syms_def by auto
+      ultimately show ?thesis
+        by blast
     qed
+    ultimately show ?thesis by fast
+  next
+    assume "(A, w) \<in> new"
+    with assms(3) u have "nts_of_syms (map Tm u' @ [Nt A] @ v') \<inter> Lhss new = {}" by simp
+    then have "nts_of_syms [Nt A] \<inter> Lhss new = {}"
+      unfolding nts_of_syms_def by auto
+    then have "A \<notin> Lhss new" unfolding nts_of_syms_def by auto
+    with \<open>(A, w) \<in> new\<close> have False unfolding Lhss_def by auto
+    then show ?thesis by fast
+  qed
+qed
+
+
+
+(* helper for append_unreachable_productions_derives *)
+lemma append_unreachable_productions_derive:
+  assumes "old \<union> new \<turnstile> u \<Rightarrow> v"
+      and "Nts old \<inter> Lhss new = {}"
+      and "nts_of_syms u \<inter> Lhss new = {}"
+    shows "old \<turnstile> u \<Rightarrow> v \<and> nts_of_syms v \<inter> Lhss new = {}"
+proof -
+  thm derivel_iff
+  from assms(1) have "(\<exists>(A, w)\<in>(old \<union> new). \<exists>u1 u2. u = u1 @ Nt A # u2 \<and> v = u1 @ w @ u2)"
+    by (simp only: derive_iff)
+  then obtain A w u' v' where
+        A_w: "(A, w)\<in>(old \<union> new)"
+      and u: "u = u' @ Nt A # v'"
+      and v: "v = u' @ w @ v'"
+    by fast
+  then have "(A,w) \<in> old \<or> (A,w) \<in> new" by simp
+  then show ?thesis
+  proof (elim disjE)
+    assume "(A, w) \<in> old"
+    with u v have "(A, w) \<in> old"
+        and u: "u = u' @ Nt A # v'"
+        and v: "v = u' @ w @ v'" by auto
+    then have "old \<turnstile> u \<Rightarrow> v" using derive.intros by fastforce
+    moreover have "nts_of_syms v \<inter> Lhss new = {}"
+    proof -
+      from v have "nts_of_syms v = nts_of_syms u' \<union> nts_of_syms w \<union> nts_of_syms v'"
+        unfolding nts_of_syms_def by auto
+      moreover from \<open>(A, w) \<in> old\<close> have "nts_of_syms w \<subseteq> Nts old"
+        unfolding nts_of_syms_def Nts_def by auto
+      with assms have "nts_of_syms w \<inter> Lhss new = {}"
+        by fast
+      moreover from u assms have "nts_of_syms u' \<inter> Lhss new = {}"
+        unfolding nts_of_syms_def by auto
+      moreover from u assms have "nts_of_syms v' \<inter> Lhss new = {}"
+        unfolding nts_of_syms_def by auto
+      ultimately show ?thesis
+        by blast
+    qed
+    ultimately show ?thesis by fast
+  next
+    assume "(A, w) \<in> new"
+    with assms(3) u have "nts_of_syms (u' @ [Nt A] @ v') \<inter> Lhss new = {}" by simp
+    then have "nts_of_syms [Nt A] \<inter> Lhss new = {}"
+      unfolding nts_of_syms_def by auto
+    then have "A \<notin> Lhss new" unfolding nts_of_syms_def by auto
+    with \<open>(A, w) \<in> new\<close> have False unfolding Lhss_def by auto
+    then show ?thesis by fast
+  qed
+qed
+
+
+
+lemma append_unreachable_productions_deriveln:
+  assumes "old \<union> new \<turnstile> u \<Rightarrow>l(n) v"
+      and "Nts old \<inter> Lhss new = {}"
+      and "nts_of_syms u \<inter> Lhss new = {}"
+    shows "old \<turnstile> u \<Rightarrow>l(n) v \<and> nts_of_syms v \<inter> Lhss new = {}"
+proof -
+  from assms show "old \<turnstile> u \<Rightarrow>l(n) v \<and> nts_of_syms v \<inter> Lhss new = {}"
+  proof (induction n arbitrary: v)
+    case 0
+    then show ?case by simp
+  next
+    case (Suc n')
+    then obtain v' where split: "old \<union> new \<turnstile> u \<Rightarrow>l(n') v' \<and> old \<union> new \<turnstile> v' \<Rightarrow>l v"
+      by (meson relpowp_Suc_E)
+    with Suc have "old \<turnstile> u \<Rightarrow>l(n') v' \<and> nts_of_syms v' \<inter> Lhss new = {}"
+      by fast
+    with Suc show ?case using append_unreachable_productions_derivel
+      by (metis split relpowp_Suc_I)
   qed
 qed
 
 
 (* If two grammars with disjoint sets of nonterminals are merged, 
-   then words derived from words which only contain nonterminals
-   of one grammar can also contain only such nonterminals.
+   then words derived in the merged grammar 
+   from words which only contain nonterminals of one grammar
+   can also be derived in the other grammar.
  *)
-lemma append_unreachable_productions_derive:
-  assumes "old \<union> new \<turnstile> u \<Rightarrow>* v"
+lemma append_unreachable_productions_deriven:
+  assumes "old \<union> new \<turnstile> u \<Rightarrow>(n) v"
       and "Nts old \<inter> Lhss new = {}"
-      and "nts_of_syms u \<subseteq> Nts old"
-    shows "nts_of_syms v \<subseteq> Nts old"
+      and "nts_of_syms u \<inter> Lhss new = {}"
+    shows "old \<turnstile> u \<Rightarrow>(n) v \<and> nts_of_syms v \<inter> Lhss new = {}"
 proof -
-  from assms show "nts_of_syms v \<subseteq> Nts old"
-  proof (induction rule: derives_induct')
-    case base
-    then show ?case by auto
+  from assms show "old \<turnstile> u \<Rightarrow>(n) v \<and> nts_of_syms v \<inter> Lhss new = {}"
+  proof (induction n arbitrary: v)
+    case 0
+    then show ?case by simp
   next
-    case (step u' A v' w)
-
-    from \<open>(A, w) \<in> old \<union> new\<close> have "(A,w) \<in> old \<or> (A,w) \<in> new" by simp
-    then show ?case
-    proof (elim disjE)
-      assume "(A, w) \<in> old"
-      then have "nts_of_syms w \<subseteq> Nts old" unfolding nts_of_syms_def Nts_def by fast
-      with step(5) have "nts_of_syms (u' @ w @ v') \<subseteq> Nts old" unfolding nts_of_syms_def by auto
-      with step(4) step(3) show "nts_of_syms v \<subseteq> Nts old" by fast
-    next
-      assume "(A, w) \<in> new"
-
-      from \<open>nts_of_syms (u' @ [Nt A] @ v') \<subseteq> Nts old\<close> have "nts_of_syms [Nt A] \<subseteq> Nts old"
-        unfolding nts_of_syms_def by auto
-      then have "A \<in> Nts old" unfolding nts_of_syms_def by simp
-      then have "A \<notin> Lhss new" using \<open>Nts old \<inter> Lhss new = {}\<close> by auto
-      with \<open>(A, w) \<in> new\<close> have False unfolding Lhss_def by auto
-      then show "nts_of_syms v \<subseteq> Nts old" by fast
-    qed
+    case (Suc n')
+    then obtain v' where split: "old \<union> new \<turnstile> u \<Rightarrow>(n') v' \<and> old \<union> new \<turnstile> v' \<Rightarrow> v"
+      by (meson relpowp_Suc_E)
+    with Suc have "old \<turnstile> u \<Rightarrow>(n') v' \<and> nts_of_syms v' \<inter> Lhss new = {}"
+      by fast
+    with Suc show ?case using append_unreachable_productions_derive
+      by (metis split relpowp_Suc_I)
   qed
 qed
+
+
+lemma append_unreachable_productions_derivel_iff:
+  assumes "Nts old \<inter> Lhss new = {}"
+      and "nts_of_syms u \<subseteq> Nts old"
+    shows "old \<turnstile> u \<Rightarrow>l v \<longleftrightarrow> old \<union> new \<turnstile> u \<Rightarrow>l v"
+proof
+  assume "old \<turnstile> u \<Rightarrow>l v"
+  then show "old \<union> new \<turnstile> u \<Rightarrow>l v" by (simp add: Un_derivel)
+next
+  assume "old \<union> new \<turnstile> u \<Rightarrow>l v"
+  with assms show "old \<turnstile> u \<Rightarrow>l v"
+    using append_unreachable_productions_derivel by fast
+qed
+
+lemma append_unreachable_productions_derive_iff:
+  assumes "Nts old \<inter> Lhss new = {}"
+      and "nts_of_syms u \<subseteq> Nts old"
+    shows "old \<turnstile> u \<Rightarrow> v \<longleftrightarrow> old \<union> new \<turnstile> u \<Rightarrow> v"
+proof
+  assume "old \<turnstile> u \<Rightarrow> v"
+  then show "old \<union> new \<turnstile> u \<Rightarrow> v" by (simp add: Un_derive)
+next
+  assume "old \<union> new \<turnstile> u \<Rightarrow> v"
+  with assms show "old \<turnstile> u \<Rightarrow> v"
+    using append_unreachable_productions_derive by fast
+qed
+
+
+lemma append_unreachable_productions_deriveln_iff:
+  assumes "Nts old \<inter> Lhss new = {}"
+      and "nts_of_syms u \<inter> Lhss new = {}"
+    shows "old \<turnstile> u \<Rightarrow>l(n) v \<longleftrightarrow> old \<union> new \<turnstile> u \<Rightarrow>l(n) v"
+proof
+  assume "old \<turnstile> u \<Rightarrow>l(n) v"
+  then show "old \<union> new \<turnstile> u \<Rightarrow>l(n) v"
+  proof (induction n)
+    case 0
+    then show ?case by simp
+  next
+    case (Suc n')
+    then have "\<exists>v'. old \<turnstile> u \<Rightarrow>l(n') v' \<and> old \<turnstile> v' \<Rightarrow>l v"
+      by (meson relpowp_Suc_E)
+    then show ?case using Un_derivel
+      by (metis Suc.prems relpowp_mono)
+  qed
+next
+  assume "old \<union> new \<turnstile> u \<Rightarrow>l(n) v"
+  then show "old \<turnstile> u \<Rightarrow>l(n) v"
+    using assms by (simp only: append_unreachable_productions_deriveln)
+qed
+
+
+lemma append_unreachable_productions_deriven_iff:
+  assumes "Nts old \<inter> Lhss new = {}"
+      and "nts_of_syms u \<inter> Lhss new = {}"
+    shows "old \<turnstile> u \<Rightarrow>(n) v \<longleftrightarrow> old \<union> new \<turnstile> u \<Rightarrow>(n) v"
+proof
+  assume "old \<turnstile> u \<Rightarrow>(n) v"
+  then show "old \<union> new \<turnstile> u \<Rightarrow>(n) v"
+  proof (induction n)
+    case 0
+    then show ?case by simp
+  next
+    case (Suc n')
+    then have "\<exists>v'. old \<turnstile> u \<Rightarrow>(n') v' \<and> old \<turnstile> v' \<Rightarrow> v"
+      by (meson relpowp_Suc_E)
+    then show ?case using Un_derive
+      by (metis Suc.prems relpowp_mono)
+  qed
+next
+  assume "old \<union> new \<turnstile> u \<Rightarrow>(n) v"
+  then show "old \<turnstile> u \<Rightarrow>(n) v"
+    using assms by (simp only: append_unreachable_productions_deriven)
+qed
+
+
 
 
 (* If two grammars with disjoint sets of nonterminals are merged, 
@@ -93,61 +365,25 @@ qed
 lemma append_unreachable_productions_L:
   assumes "Nts old \<inter> Lhss new = {}"
   and "S \<notin> Lhss new"
-  shows "Lang old S = Lang (old \<union> new) S"
-proof
-  show "Lang old S \<subseteq> Lang (old \<union> new) S"
-  proof
-    fix x
-    assume "x \<in> Lang old S"
-    then have "old \<turnstile> [Nt S] \<Rightarrow>* map Tm x" unfolding Lang_def by simp
-    then have "old \<union> new \<turnstile> [Nt S] \<Rightarrow>* map Tm x"
-      by (metis (no_types, opaque_lifting) Un_derive mono_rtranclp)
-    then show "x \<in> Lang (old \<union> new) S" unfolding Lang_def by simp
-  qed
+shows "Lang old S = Lang (old \<union> new) S"
+proof (cases "S \<in> Lhss old")
+  case True
+  with assms have "S \<notin> Lhss new" by fast
+
+  then have "nts_of_syms [Nt S] \<inter> Lhss new = {}" unfolding nts_of_syms_def Lhss_def
+    by simp
+  from assms(1) this have "\<And>n v. (old \<turnstile> [Nt S] \<Rightarrow>(n) v) = (old \<union> new \<turnstile> [Nt S] \<Rightarrow>(n) v)"
+    by (rule append_unreachable_productions_deriven_iff)
+  then show ?thesis unfolding Lang_def
+    by (simp add: rtranclp_power)
 next
-  show "Lang (old \<union> new) S \<subseteq> Lang old S"
-  proof
-    fix x
-    assume "x \<in> Lang (old \<union> new) S"
-    then have "old \<union> new \<turnstile> [Nt S] \<Rightarrow>* map Tm x" unfolding Lang_def by simp
-    then have "old \<turnstile> [Nt S] \<Rightarrow>* map Tm x"
-    proof (induction)
-      case base
-      then show ?case by simp
-    next
-      case (step y z)
-      from step(2) have derivations: "old \<turnstile> y \<Rightarrow> z \<or> new \<turnstile> y \<Rightarrow> z" by (simp only: Un_derive)
-      show ?case
-      proof (cases "old \<turnstile> y \<Rightarrow> z")
-        case True
-        then show ?thesis
-          using step.IH by simp 
-      next
-        case False
-        with derivations have "new \<turnstile> y \<Rightarrow> z" by simp
-        then have "(\<exists> (A,w) \<in> new. \<exists>u1 u2. y = u1 @ Nt A # u2 \<and> z = u1 @ w @ u2)" by (simp only: derive_iff)
-        then obtain A w u1 u2 where y_A: "(A,w) \<in> new \<and> y = u1 @ Nt A # u2 \<and> z = u1 @ w @ u2" by fast
-        then have A_new: "A \<in> Lhss new" unfolding Lhss_def by auto
-
-        from \<open>old \<turnstile> [Nt S] \<Rightarrow>* y\<close> have "nts_of_syms y \<subseteq> Nts old \<union> nts_of_syms [Nt S]"
-          using nts_prods_subset sorry (* ? ? *)
-      (*
-        from nts_prods_subset[where u="[Nt S]" and v=y and P=old]
-        have x: "old \<turnstile> [Nt S] \<Rightarrow>* y \<Longrightarrow> nts_of_syms y \<subseteq> Nts old \<union> nts_of_syms [Nt S]" by simp
-  
-        print_statement nts_prods_subset[where u="[Nt S]" and v=y and P=old]
-        print_statement x
-      *)
-
-        then have "nts_of_syms y \<subseteq> Nts old \<union> {S}" unfolding nts_of_syms_def by simp
-        moreover from y_A have "A \<in> nts_of_syms y" unfolding nts_of_syms_def by simp
-        ultimately have "A \<in> Nts old \<union> {S}" by auto
-        with A_new assms have False by auto
-        then show ?thesis by simp
-      qed
-    qed
-    then show " x \<in> Lang old S" unfolding Lang_def by simp
-  qed
+  case False
+  then have "Lang old S = {}"
+    by (simp add: Lang_empty_if_notin_Lhss)
+  moreover from False assms(2) have "S \<notin> Lhss (old \<union> new)" unfolding Lhss_def by auto
+  then have "Lang (old \<union> new) S = {}"
+    by (simp add: Lang_empty_if_notin_Lhss) 
+  ultimately show ?thesis by fast
 qed
 
 
