Gschossmann/cnf_induct.thy
@@ -1,0 +1,38 @@
+theory cnf_induct
+  imports "../Stimpfle/CNF" "derivel_nts"
+begin
+
+(* custom induction rule for leftmost derivations in CNF *)
+lemma cnf_derivels_induct[consumes 2, case_names base step_nt_nt step_tm]:
+  assumes "P \<turnstile> xs \<Rightarrow>l* ys"
+  and cnf: "CNF P"
+  and Base: "Q ys"
+  and Step1: "\<And>u A v B C. \<lbrakk> P \<turnstile> map Tm u @ [Nt A] @ v \<Rightarrow>l* ys; Q (map Tm u @ [Nt B,Nt C] @ v); (A,[Nt B,Nt C]) \<in> P \<rbrakk> \<Longrightarrow> Q (map Tm u @ [Nt A] @ v)"
+  and Step2: "\<And>u A v t. \<lbrakk> P \<turnstile> map Tm u @ [Nt A] @ v \<Rightarrow>l* ys; Q (map Tm u @ [Tm t] @ v); (A,[Tm t]) \<in> P \<rbrakk> \<Longrightarrow> Q (map Tm u @ [Nt A] @ v)"
+  shows "Q xs"
+  using assms(1)
+proof (induction rule: converse_rtranclp_induct)
+  case base
+  then show ?case using Base by fast
+next
+  case (step y z)
+  then have "(\<exists> (A,w) \<in> P. \<exists>u1 u2. y = map Tm u1 @ Nt A # u2 \<and> z = map Tm u1 @ w @ u2)"
+    by (simp only: derivel_iff)
+  then obtain A w u1 u2 where split: "(A,w) \<in> P \<and> y = map Tm u1 @ Nt A # u2 \<and> z = map Tm u1 @ w @ u2"
+    by fast
+  with cnf have "(\<exists>B C. w = [Nt B, Nt C]) \<or> (\<exists>t. w = [Tm t])" unfolding CNF_def by fast
+  then show ?case
+  proof (elim disjE)
+    assume "\<exists>B C. w = [Nt B, Nt C]"
+    then obtain B C where "w = [Nt B, Nt C]" by fast
+    with split step Step1 show "Q y" 
+      by (simp add: converse_rtranclp_into_rtranclp derivels_imp_derives)
+  next
+    assume "\<exists>t. w = [Tm t]"
+    then obtain t where "w = [Tm t]" by fast
+    with split step Step2 show "Q y" 
+      by (simp add: converse_rtranclp_into_rtranclp derivels_imp_derives)
+  qed
+qed
+
+end
